assertions.v
@@ -1,0 +1,636 @@
+(* Copyright (c) 2012-2015, Robbert Krebbers. *)
+(* This file is distributed under the terms of the BSD license. *)
+(** We define assertions of Hoare logic using a shallow embedding. That is,
+assertions are predicates over the contents of the stack and memory. *)
+
+(** This file defines the data type of assertions, the usual connectives of
+Hoare logic ([∧], [¬], [↔], [∀] and [∃]), the connectives of separation
+logic ([emp], [↦], [★]), and other connectives that are more specific to
+our development. We overload the usual notations in [assert_scope] to obtain
+nicely looking assertions. *)
+Require Export expression_eval type_system memory_separation.
+Local Obligation Tactic := idtac.
+
+Local Hint Extern 1 (_ ⊆ _) => etransitivity; [eassumption|].
+Local Hint Extern 1 (_ ⊆ _) => etransitivity; [|eassumption].
+Local Hint Extern 1 (_ ⇒ₘ _) => etransitivity; [|eassumption].
+Local Hint Extern 1 (_ ⇒ₘ _) => etransitivity; [|eassumption].
+Local Hint Extern 1 (_ ⊆{_} _) => etransitivity; [eassumption|].
+Local Hint Extern 1 (_ ⊆{_} _) => etransitivity; [|eassumption].
+
+(** * Definition of assertions *)
+Record assert (K : Set) `{Env K} := Assert {
+  assert_holds : env K → memenv K → stack → list (type K) → mem K → Prop;
+  assert_weaken Γ1 Γ2 Δ1 Δ2 ρ τs m :
+    ✓ Γ1 → ✓{Γ1,Δ1} m → Δ1 ⊢* ρ :* τs →
+    assert_holds Γ1 Δ1 ρ τs m →
+    Γ1 ⊆ Γ2 → Δ1 ⇒ₘ Δ2 →
+    assert_holds Γ2 Δ2 ρ τs m
+}.
+Add Printing Constructor assert.
+
+Delimit Scope assert_scope with A.
+Bind Scope assert_scope with assert.
+Arguments Assert {_ _} _ _.
+Arguments assert_holds {_ _} _%A _ _ _ _ _.
+Arguments assert_weaken {_ _} _%A _ _ _ _ _ _ _ _ _ _ _ _ _.
+
+(** The relation [P ⊆@{Γ} Q] states that the assertion [Q] is a logical
+consequence of [P] in [Γ] and [P ≡@{Γ} Q] states that [P] and [Q] are logically
+equivalent in [Γ]. *)
+Instance assert_entails `{Env K} : SubsetEqE (env K) (assert K) := λ Γ P Q,
+  ∀ Γ' Δ ρ τs m,
+    Γ ⊆ Γ' → ✓ Γ' → ✓{Γ',Δ} m → Δ ⊢* ρ :* τs →
+    assert_holds P Γ' Δ ρ τs m → assert_holds Q Γ' Δ ρ τs m.
+Instance assert_equiv `{Env K} : EquivE (env K) (assert K) := λ Γ P Q,
+  P ⊆{Γ} Q ∧ Q ⊆{Γ} P.
+
+(** * Hoare logic connectives *)
+(** Definitions and notations of the usual connectives of Hoare logic. *)
+Program Definition assert_Prop `{Env K} (P : Prop) : assert K := {|
+  assert_holds := λ _ _ _ _ m, P ∧ m = ∅
+|}.
+Next Obligation. naive_solver. Qed.
+Notation "⌜ P ⌝" := (assert_Prop P) (format "⌜  P  ⌝") : assert_scope.
+Notation "'False'" := (assert_Prop False) : assert_scope.
+
+Program Definition assert_impl `{Env K} (P Q : assert K) : assert K := {|
+  assert_holds := λ Γ Δ ρ τs m, ∀ Γ' Δ',
+    Γ ⊆ Γ' → ✓ Γ' → Δ ⇒ₘ Δ' → ✓{Γ',Δ'} m →
+    assert_holds P Γ' Δ' ρ τs m → assert_holds Q Γ' Δ' ρ τs m
+|}.
+Next Obligation.
+  intros ?? P Q Γ1 Γ2 Δ1 Δ2 ρ τs m ??? HPQ ?? Γ3 Δ3 ?????.
+  apply HPQ; eauto.
+Qed.
+Infix "→" := assert_impl : assert_scope.
+Notation "(→)" := assert_impl (only parsing) : assert_scope.
+Notation "( P →)" := (assert_impl P) (only parsing) : assert_scope.
+Notation "(→ Q )" := (λ P, assert_impl P Q) (only parsing) : assert_scope.
+
+Program Definition assert_and `{Env K} (P Q : assert K) : assert K := {|
+  assert_holds := λ Γ Δ ρ τs m,
+    assert_holds P Γ Δ ρ τs m ∧ assert_holds Q Γ Δ ρ τs m
+|}.
+Next Obligation. naive_solver eauto using assert_weaken. Qed.
+Infix "∧" := assert_and : assert_scope.
+Notation "(∧)" := assert_and (only parsing) : assert_scope.
+Notation "( P ∧)" := (assert_and P) (only parsing) : assert_scope.
+Notation "(∧ Q )" := (λ P, assert_and P Q) (only parsing) : assert_scope.
+
+Definition assert_not `{Env K} (P : assert K) : assert K := (P → False)%A.
+Notation "¬ P" := (assert_not P) : assert_scope.
+Definition assert_iff `{Env K} (P Q : assert K) : assert K :=
+  ((P → Q) ∧ (Q → P))%A.
+Infix "↔" := assert_iff : assert_scope.
+Notation "(↔)" := assert_iff (only parsing) : assert_scope.
+Notation "( P ↔)" := (assert_iff P) (only parsing) : assert_scope.
+Notation "(↔ Q )" := (λ P, assert_iff P Q) (only parsing) : assert_scope.
+
+Program Definition assert_forall `{Env K} `(P: A → assert K) : assert K := {|
+  assert_holds := λ Γ Δ ρ τs m, ∀ x, assert_holds (P x) Γ Δ ρ τs m
+|}.
+Next Obligation. naive_solver eauto using assert_weaken. Qed.
+Notation "∀ x .. y , P" :=
+  (assert_forall (λ x, .. (assert_forall (λ y, P)) ..)) : assert_scope.
+
+Program Definition assert_exist `{Env K} `(P : A → assert K): assert K := {|
+  assert_holds := λ Γ Δ ρ τs m, ∃ x, assert_holds (P x) Γ Δ ρ τs m
+|}.
+Next Obligation. naive_solver eauto using assert_weaken. Qed.
+Notation "∃ x .. y , P" :=
+  (assert_exist (λ x, .. (assert_exist (λ y, P)) ..)) : assert_scope.
+
+(** * Separation logic connectives *)
+(** The assertion [emp] asserts that the memory is empty. The assertion [P ★ Q]
+(called separating conjunction) asserts that the memory can be split into two
+disjoint parts such that [P] holds in the one part, and [Q] in the other. *)
+Notation "'emp'" := (assert_Prop True) : assert_scope.
+
+Program Definition assert_sep `{EnvSpec K} (P Q : assert K) : assert K := {|
+  assert_holds := λ Γ Δ ρ τs m, ∃ m1 m2,
+    m = m1 ∪ m2 ∧ ⊥[m1; m2] ∧
+    assert_holds P Γ Δ ρ τs m1 ∧ assert_holds Q Γ Δ ρ τs m2
+|}.
+Next Obligation.
+  intros ??? P Q Γ1 Γ2 Δ1 Δ2 ρ τs m ??? (m1&m2&->&?&?&?) ??.
+  eauto 15 using assert_weaken, cmap_valid_subseteq,
+    (@sep_union_subseteq_l (mem K) _ _), (@sep_union_subseteq_r (mem K) _ _).
+Qed.
+Infix "★" := assert_sep (at level 80, right associativity) : assert_scope.
+Notation "(★)" := assert_sep (only parsing) : assert_scope.
+Notation "( P ★)" := (assert_sep P) (only parsing) : assert_scope.
+Notation "(★ Q )" := (λ P, assert_sep P Q) (only parsing) : assert_scope.
+
+(** The assertion [Π Ps] states that the memory can be split into disjoint
+parts such that for each part the corresponding assertion in [Ps] holds. *)
+Definition assert_sep_list `{EnvSpec K} :
+  list (assert K) → assert K := foldr (★)%A emp%A.
+Notation "'Π' Ps" := (assert_sep_list Ps)
+  (at level 20, format "Π  Ps") : assert_scope.
+
+(** The assertion [e ⇓ v : τlr] asserts that the expression [e] evaluates to [v]
+and [e ⇓ - : τlr] asserts that the expression [e] evaluates to an arbitrary
+value (in other words, [e] does not impose undefined behavior). *)
+Notation vassert K := (lrval K → assert K).
+Program Definition assert_expr `{EnvSpec K}
+    (e : expr K) (τlr : lrtype K) : vassert K := λ av, {|
+  assert_holds := λ Γ Δ ρ τs m, (Γ,Δ,τs) ⊢ e : τlr ∧ ⟦ e ⟧ Γ ∅ ρ m = Some av
+|}.
+Next Obligation.
+  intros ??? e τlr av Γ1 Γ2 Δ1 Δ2 ρ τs m ??? [??] ??; split;
+    eauto using expr_typed_weaken, expr_eval_weaken, purefuns_empty_valid,
+    mem_lookup_weaken, mem_forced_weaken.
+Qed.
+Notation "e ⇓ av : τlr" := (assert_expr e τlr av)%A
+  (at level 60, av at next level, τlr at next level,
+   format "e  '⇓'  av  :  τlr") : assert_scope.
+Notation "e ⇓ - : τlr" := (∃ av, e ⇓ av : τlr)%A
+  (at level 60, τlr at next level,
+   format "e  '⇓'  '-'  :  τlr") : assert_scope.
+
+(** The assertion [e1 ↦{malloc,x} e2] asserts that the memory consists of
+exactly one object at address [e1] with permission [x] and contents [e2]. The
+assertion [e1 ↦{malloc,x} -] asserts that the memory consists of exactly one
+object at address [e1] with permission [x] and arbitrary contents. The Boolean
+[malloc] denotes whether the object has been obtained via malloc. *)
+Program Definition assert_singleton `{EnvSpec K}
+    (e1 e2 : expr K) (malloc : bool) (x : perm) (τ : type K) : assert K := {|
+  assert_holds := λ Γ Δ ρ τs m, ∃ a v,
+    (Γ,Δ,τs) ⊢ e1 : inl τ ∧ ⟦ e1 ⟧ Γ ∅ ρ ∅ = Some (inl a) ∧
+    (Γ,Δ,τs) ⊢ e2 : inr τ ∧ ⟦ e2 ⟧ Γ ∅ ρ ∅ = Some (inr v) ∧
+    addr_is_obj a ∧ sep_valid x ∧ ¬sep_unmapped x ∧ 
+    m = mem_singleton Γ a malloc x v
+|}.
+Next Obligation.
+  intros ??? e1 e2 ml x τ Γ1 Γ2 Δ1 Δ2 ρ τs m ??? (a&v&?&?&?&?&?&?&?&->) ??.
+  exists a v; split_ands;
+    eauto 15 using expr_typed_weaken, expr_eval_weaken_empty,
+    purefuns_empty_valid, mem_singleton_weaken, cmap_valid_memenv_valid,
+    lval_typed_inv, lval_typed_strict, rval_typed_inv, expr_eval_typed,
+    cmap_empty_valid.
+Qed.
+Notation "e1 ↦{ malloc , x } e2 : τ" := (assert_singleton e1 e2 malloc x τ)%A
+  (at level 20, malloc at next level, x at next level, e2 at next level,
+   τ at next level, format "e1  ↦{ malloc , x }  e2  :  τ") : assert_scope.
+Notation "e1 ↦{ malloc , x } - : τ" :=
+  (∃ av, e1 ↦{malloc,x} (lrval_to_expr av) : τ)%A
+  (at level 20, malloc at next level, x at next level,
+   τ at next level, format "e1  ↦{ malloc , x }  -  :  τ") : assert_scope.
+
+(** The assertion [P ○] asserts that [P] holds if all sequenced locations
+are unlocked. *)
+Program Definition assert_unlock `{EnvSpec K} (P : assert K) : assert K := {|
+  assert_holds := λ Γ Δ ρ τs m, assert_holds P Γ Δ ρ τs (mem_unlock_all m)
+|}.
+Next Obligation.
+  naive_solver eauto using assert_weaken, mem_unlock_all_valid.
+Qed.
+Notation "P ○" := (assert_unlock P) (at level 20) : assert_scope.
+
+(** The assertion [P↡] asserts that [P] holds if the stack is cleared. This
+connective allows us to specify stack independence in an alternative way. *)
+Program Definition assert_clear_stack `{Env K} (P : assert K) : assert K := {|
+  assert_holds := λ Γ Δ ρ τs m, assert_holds P Γ Δ [] [] m
+|}.
+Next Obligation. naive_solver eauto using assert_weaken. Qed.
+Notation "P ↡" := (assert_clear_stack P) (at level 20) : assert_scope.
+
+(** To deal with block scope variables we need to lift an assertion such that
+the De Bruijn indexes of its variables are increased. We define the lifting
+[P↑] of an assertion [P] semantically, and prove that it indeed behaves as
+expected. *)
+Program Definition assert_lift `{Env K} (P : assert K) : assert K := {|
+  assert_holds := λ Γ Δ ρ τs m, assert_holds P Γ Δ (tail ρ) (tail τs) m
+|}.
+Next Obligation. naive_solver eauto using assert_weaken, Forall2_tail. Qed.
+Notation "P ↑" := (assert_lift P) (at level 20) : assert_scope.
+
+(** * Subclasses of assertions *)
+(** The following type classes collect important subclasses of assertions.
+- [StackIndep] collects assertions that are independent of the stack.
+- [UnlockIndep] collects assertions that are independent of unlocking
+  sequenced locations in the memory.
+
+This file contains instances of these type classes for the various connectives.
+We use instance resolution to automatically compose these instances to prove
+the above properties for composite assertions. *)
+Class StackIndep `{Env K} (P : assert K) : Prop :=
+  stack_indep Γ Δ ρ1 τs1 ρ2 τs2 m :
+    ✓ Γ → ✓{Γ,Δ} m → Δ ⊢* ρ1 :* τs1 → Δ ⊢* ρ2 :* τs2 →
+    assert_holds P Γ Δ ρ1 τs1 m →
+    assert_holds P Γ Δ ρ2 τs2 m.
+Class UnlockIndep `{Env K} (P : assert K) : Prop :=
+  unlock_indep Γ Δ ρ τs m :
+    ✓ Γ → ✓{Γ,Δ} m → Δ ⊢* ρ :* τs →
+    assert_holds P Γ Δ ρ τs m →
+    assert_holds P Γ Δ ρ τs (mem_unlock_all m).
+
+Hint Extern 10 (StackIndep _) => apply _.
+Hint Extern 10 (UnlockIndep _) => apply _.
+
+Section assertions.
+Context `{EnvSpec K}.
+Implicit Types Γ : env K.
+
+Hint Unfold Proper respectful pointwise_relation : assert.
+Hint Unfold subseteqE assert_entails equivE assert_equiv : assert.
+Hint Unfold StackIndep UnlockIndep : assert.
+Hint Extern 100 (⊥ _) => solve_sep_disjoint.
+Hint Extern 100 (sep_valid _) =>
+  apply sep_disjoint_list_singleton; solve_sep_disjoint.
+Hint Immediate cmap_valid_sep_valid.
+Hint Immediate purefuns_empty_valid.
+Hint Extern 0 (Separation _) => apply (_ : Separation (mem K)).
+Hint Extern 0 (Separation _) => apply (_ : Separation perm).
+
+Ltac solve t :=
+  repeat first
+  [ progress simplify_equality'
+  | progress autounfold with assert in *];
+  naive_solver t.
+
+(** Ordinary logic connections *)
+Global Instance: PreOrder (⊆{Γ}).
+Proof. split; solve eauto. Qed.
+Global Instance: Equivalence (≡{Γ}).
+Proof. split; red; solve eauto. Qed.
+Global Instance: Proper ((≡{Γ}) ==> (≡{Γ}) ==> iff) (⊆{Γ}).
+Proof. solve eauto. Qed.
+Global Instance: Proper (impl ==> (⊆{Γ})) assert_Prop.
+Proof. solve eauto. Qed.
+Global Instance: Proper (iff ==> (≡{Γ})) assert_Prop.
+Proof. solve eauto. Qed.
+Global Instance: Proper (flip (⊆{Γ}) ==> (⊆{Γ}) ==> (⊆{Γ})) (→)%A.
+Proof.
+  intros Γ1 P1 P2 HP Q1 Q2 HQ Γ2 Δ ρ τs m ???? HPQ Γ3 Δ2 ???? HP2.
+  eapply HQ; eauto using Forall2_impl, memenv_forward_typed.
+  eapply HPQ; eauto.
+  eapply HP; eauto using Forall2_impl, memenv_forward_typed.
+Qed.
+Global Instance: Proper ((≡{Γ}) ==> (≡{Γ}) ==> (≡{Γ})) (→)%A.
+Proof. by intros ??? [??] ?? [??]; split; f_equiv. Qed.
+Global Instance: Proper ((≡{Γ}) ==> (≡{Γ}) ==> (≡{Γ})) (∧)%A.
+Proof. solve eauto. Qed.
+Global Instance: Proper ((⊆{Γ}) ==> (⊆{Γ}) ==> (⊆{Γ})) (∧)%A.
+Proof. solve eauto. Qed.
+Global Instance: Proper ((≡{Γ}) ==> (≡{Γ}) ==> (≡{Γ})) (↔)%A.
+Proof. by intros ???????; unfold assert_iff; do 2 f_equiv. Qed.
+Global Instance: Proper ((≡{Γ}) ==> (≡{Γ})) assert_not.
+Proof. by intros ????; unfold assert_not; f_equiv. Qed.
+Global Instance: Proper (flip (⊆{Γ}) ==> (⊆{Γ})) assert_not.
+Proof. by intros ????; unfold assert_not; f_equiv. Qed.
+Global Instance:
+  Proper (pointwise_relation _ (≡{Γ}) ==> (≡{Γ})) (@assert_forall _ _ A).
+Proof. solve eauto. Qed.
+Global Instance:
+  Proper (pointwise_relation _ (⊆{Γ}) ==> (⊆{Γ})) (@assert_forall _ _ A).
+Proof. solve eauto. Qed.
+Global Instance:
+  Proper (pointwise_relation _ (≡{Γ}) ==> (≡{Γ})) (@assert_exist _ _ A).
+Proof. solve eauto. Qed.
+Global Instance:
+  Proper (pointwise_relation _ (⊆{Γ}) ==> (⊆{Γ})) (@assert_exist _ _ A).
+Proof. solve eauto. Qed.
+Global Instance:
+  Proper (pointwise_relation _ (flip (⊆{Γ})) ==> (flip (⊆{Γ})))
+  (@assert_exist _ _ A).
+Proof. solve eauto. Qed.
+
+Global Instance assert_Prop_stack_indep P : StackIndep (⌜ P ⌝).
+Proof. solve eauto. Qed.
+Global Instance assert_impl_stack_indep :
+  StackIndep P → StackIndep Q → StackIndep (P → Q).
+Proof.
+  intros P Q HP HQ Γ Δ ρ1 τs1 ρ2 τs2 m ???? HPQ Γ2 Δ2 ???? HP'.
+  eapply HQ, HPQ, HP with ρ2 τs2; eauto using Forall2_impl,memenv_forward_typed.
+Qed.
+Global Instance assert_and_stack_indep :
+  StackIndep P → StackIndep Q → StackIndep (P ∧ Q).
+Proof. solve eauto. Qed.
+Global Instance assert_forall_stack_indep A :
+  (∀ x : A, StackIndep (P x)) → StackIndep (assert_forall P).
+Proof. solve eauto. Qed.
+Global Instance assert_exist_stack_indep A :
+  (∀ x : A, StackIndep (P x)) → StackIndep (assert_exist P).
+Proof. solve eauto. Qed.
+
+Global Instance assert_Prop_unlock_indep P : UnlockIndep (⌜ P ⌝).
+Proof. solve ltac:(eauto using mem_unlock_all_empty). Qed.
+Global Instance assert_and_unlock_indep :
+  UnlockIndep P → UnlockIndep Q → UnlockIndep (P ∧ Q).
+Proof. solve eauto. Qed.
+Global Instance assert_forall_unlock_indep A :
+  (∀ x : A, UnlockIndep (P x)) → UnlockIndep (assert_forall P).
+Proof. solve eauto. Qed.
+Global Instance assert_exist_unlock_indep A :
+  (∀ x : A, UnlockIndep (P x)) → UnlockIndep (assert_exist P).
+Proof. solve eauto. Qed.
+
+Global Instance: Commutative (≡{Γ}) (↔)%A.
+Proof. red; solve eauto. Qed.
+Global Instance: Commutative (≡{Γ}) (∧)%A.
+Proof. red; solve eauto. Qed.
+Global Instance: Associative (≡{Γ}) (∧)%A.
+Proof. red; solve eauto. Qed.
+Global Instance: Idempotent (≡{Γ}) (∧)%A.
+Proof. red; solve eauto. Qed.
+Global Instance: LeftAbsorb (≡{Γ}) False%A (∧)%A.
+Proof. red; solve eauto. Qed.
+Global Instance: RightAbsorb (≡{Γ}) False%A (∧)%A.
+Proof. red; solve eauto. Qed.
+Lemma assert_Prop_impl Γ (P Q : Prop) : ⌜ P → Q ⌝%A ⊆{Γ} (⌜P⌝ → ⌜Q⌝)%A.
+Proof. solve eauto. Qed.
+Lemma assert_Prop_not Γ (P : Prop) : ⌜ ¬P ⌝%A ⊆{Γ} (¬⌜P⌝)%A.
+Proof. apply assert_Prop_impl. Qed.
+Lemma assert_Prop_and Γ (P Q : Prop) : ⌜ P ∧ Q ⌝%A ≡{Γ} (⌜P⌝ ∧ ⌜Q⌝)%A.
+Proof. solve eauto. Qed.
+Lemma assert_false_elim Γ P : False%A ⊆{Γ} P.
+Proof. solve eauto. Qed.
+Lemma assert_and_l Γ P Q : (P ∧ Q)%A ⊆{Γ} P.
+Proof. solve eauto. Qed.
+Lemma assert_and_r Γ P Q : (P ∧ Q)%A ⊆{Γ} Q.
+Proof. solve eauto. Qed.
+Lemma assert_and_intro Γ P Q1 Q2 : P ⊆{Γ} Q1 → P ⊆{Γ} Q2 → P ⊆{Γ} (Q1 ∧ Q2)%A.
+Proof. solve eauto. Qed.
+Lemma assert_and_elim_l Γ P1 P2 Q : P1 ⊆{Γ} Q → (P1 ∧ P2)%A ⊆{Γ} Q.
+Proof. solve eauto. Qed.
+Lemma assert_and_elim_r Γ P1 P2 Q : P2 ⊆{Γ} Q → (P1 ∧ P2)%A ⊆{Γ} Q.
+Proof. solve eauto. Qed.
+Lemma assert_forall_intro {A} Γ P (Q : A → assert K) :
+  (∀ x, P ⊆{Γ} Q x) → P ⊆{Γ} (∀ x, Q x)%A.
+Proof. solve eauto. Qed.
+Lemma assert_forall_elim {A} Γ (P : A → assert K) Q x :
+  (P x ⊆{Γ} Q) → (∀ x, P x)%A ⊆{Γ} Q.
+Proof. solve eauto. Qed.
+Lemma assert_exist_intro {A} Γ P (Q : A → assert K) x :
+  P ⊆{Γ} Q x → P ⊆{Γ} (∃ x, Q x)%A.
+Proof. solve eauto. Qed.
+Lemma assert_exist_elim {A} Γ (P : A → assert K) Q :
+  (∀ x, P x ⊆{Γ} Q) → (∃ x, P x)%A ⊆{Γ} Q.
+Proof. solve eauto. Qed.
+Lemma assert_and_exist {A} Γ P (Q : A → assert K) :
+  (P ∧ ∃ x, Q x)%A ≡{Γ} (∃ x, P ∧ Q x)%A.
+Proof. solve eauto. Qed.
+Lemma assert_exist_and {A} Γ (P : A → assert K) Q :
+  ((∃ x, P x) ∧ Q)%A ≡{Γ} (∃ x, P x ∧ Q)%A.
+Proof. solve eauto. Qed.
+Lemma assert_Prop_intro_l Γ (P : Prop) Q R :
+  (P → Q ⊆{Γ} R) → (⌜ P ⌝ ∧ Q)%A ⊆{Γ} R.
+Proof. solve eauto. Qed.
+Lemma assert_Prop_intro_r Γ (P : Prop) Q R :
+  (P → Q ⊆{Γ} R) → (Q ∧ ⌜ P ⌝)%A ⊆{Γ} R.
+Proof. solve eauto. Qed.
+Lemma assert_Prop_and_elim Γ (P : Prop) Q R :
+  (P → Q ⊆{Γ} R) → (⌜ P ⌝ ∧ Q)%A ⊆{Γ} R.
+Proof. solve eauto. Qed.
+Lemma assert_and_Prop_elim Γ (P : Prop) Q R :
+  (P → Q ⊆{Γ} R) → (Q ∧ ⌜ P ⌝)%A ⊆{Γ} R.
+Proof. solve eauto. Qed.
+
+(** Separation logic connectives *)
+Global Instance: Proper ((⊆{Γ}) ==> (⊆{Γ}) ==> (⊆{Γ})) (★)%A.
+Proof.
+  solve ltac:(eauto 15 using cmap_valid_subseteq,
+    @sep_union_subseteq_l, @sep_union_subseteq_r).
+Qed.
+Global Instance: Proper ((≡{Γ}) ==> (≡{Γ}) ==> (≡{Γ})) (★)%A.
+Proof.
+  by intros ??? [??] ?? [??]; split;
+    apply (_ : Proper ((⊆{Γ}) ==> (⊆{Γ}) ==> (⊆{Γ})) (★)%A).
+Qed.
+Global Instance: Proper (Forall2 (≡{Γ}) ==> (≡{Γ})) assert_sep_list.
+Proof.
+  induction 1; simpl; [done|];
+    by apply (_ : Proper ((≡{Γ}) ==> (≡{Γ}) ==> (≡{Γ})) (★)%A).
+Qed.
+
+Global Instance assert_sep_unlock_indep P Q :
+  UnlockIndep P → UnlockIndep Q → UnlockIndep (P ★ Q).
+Proof.
+  intros HP HQ Γ Δ δ τs m ??? (m1&m2&->&?&?&?).
+  rewrite mem_unlock_all_union by solve_sep_disjoint.
+  exists (mem_unlock_all m1) (mem_unlock_all m2); split_ands;
+    rewrite <-?mem_unlock_all_disjoint_le; eauto using
+    cmap_valid_subseteq, @sep_union_subseteq_l, @sep_union_subseteq_r.
+Qed.
+Global Instance assert_sep_stack_indep :
+  StackIndep P → StackIndep Q → StackIndep (P ★ Q).
+Proof.
+  solve ltac:(eauto 15 using cmap_valid_subseteq,
+    @sep_union_subseteq_l, @sep_union_subseteq_r).
+Qed.
+
+Global Instance: Commutative (⊆{Γ}) (★)%A.
+Proof.
+  intros Γ P Q Γ1 Δ1 ρ τs m ???? (m1&m2&->&?&?&?).
+  exists m2 m1. rewrite sep_commutative by auto; auto.
+Qed.
+Global Instance: Commutative (≡{Γ}) (★)%A.
+Proof. split; by rewrite (commutative (★)%A). Qed.
+Global Instance: LeftId (≡{Γ}) emp%A (★)%A.
+Proof.
+  intros Γ; intros P; split.
+  * intros Γ1 Δ1 ρ τs m ???? (m1&m2&->&?&[_ ->]&?).
+    rewrite sep_left_id by auto; auto.
+  * intros Γ1 Δ1 ρ τs m ?????. eexists ∅, m.
+    rewrite sep_left_id, sep_disjoint_equiv_empty,
+      sep_disjoint_list_singleton by eauto; solve eauto.
+Qed.
+Global Instance: RightId (≡{Γ}) emp%A (★)%A.
+Proof. intros ??. by rewrite (commutative _), (left_id _ _). Qed.
+Global Instance: LeftAbsorb (≡{Γ}) False%A (★)%A.
+Proof. red; solve eauto. Qed.
+Global Instance: RightAbsorb (≡{Γ}) False%A (★)%A.
+Proof. red; solve eauto. Qed.
+Global Instance: Associative (≡{Γ}) (★)%A.
+Proof.
+  intros Γ. assert (∀ P Q R, ((P ★ Q) ★ R)%A ⊆{Γ} (P ★ (Q ★ R))%A).
+  { intros P Q R Γ1 Δ1 ρ τs ????? (?&m3&->&?&(m1&m2&->&?&?&?)&?).
+    exists m1 (m2 ∪ m3); rewrite sep_associative by auto; split_ands; auto.
+    exists m2 m3; auto. }
+  assert (∀ P Q R, (P ★ (Q ★ R))%A ⊆{Γ} ((P ★ Q) ★ R)%A).
+  { intros P Q R Γ1 Δ1 ρ τs ????? (m1&?&->&?&?&(m2&m3&->&?&?&?)).
+    exists (m1 ∪ m2) m3; rewrite sep_associative by auto; split_ands; auto.
+    exists m1 m2; auto. }
+  split; auto.
+Qed.
+Lemma assert_Prop_and_intro Γ (P : Prop) Q R :
+  P → Q ⊆{Γ} R → Q ⊆{Γ} (⌜ P ⌝ ★ R)%A.
+Proof.
+  intros ?? Γ1 Δ1 ρ τs ??????. eexists ∅, m.
+  rewrite sep_left_id, sep_disjoint_equiv_empty,
+    sep_disjoint_list_singleton by eauto; solve eauto.
+Qed.
+Lemma assert_and_Prop_intro Γ (P : Prop) Q R :
+  P → Q ⊆{Γ} R → Q ⊆{Γ} (R ★ ⌜ P ⌝)%A.
+Proof. rewrite (commutative (★)%A). apply assert_Prop_and_intro. Qed. 
+Lemma assert_sep_exist {A} Γ P (Q : A → assert K) :
+  (P ★ ∃ x, Q x)%A ≡{Γ} (∃ x, P ★ Q x)%A.
+Proof. solve eauto. Qed.
+Lemma assert_exist_sep {A} Γ (P : A → assert K) Q :
+  ((∃ x, P x) ★ Q)%A ≡{Γ} (∃ x, P x ★ Q)%A.
+Proof. solve eauto. Qed.
+
+(* Evaluation and singleton connectives *)
+Global Instance assert_expr_stack_indep e v τlr :
+  vars e = ∅ → StackIndep (e ⇓ v : τlr).
+Proof.
+  intros ? Γ Δ ρ1 τs1 ρ2 τs2 m ???? [??]; split;
+    erewrite 1?expr_eval_var_free by eauto; eauto using expr_typed_var_free.
+Qed.
+Global Instance assert_singleton_stack_indep e1 e2 malloc x τ :
+  vars e1 = ∅ → vars e2 = ∅ → StackIndep (e1 ↦{malloc,x} e2 : τ).
+Proof.
+  intros ?? Γ Δ ρ1 τs1 ρ2 τs2 m ???? (a&v&?&?&?&?&?&?&?&->);
+    exists a v; erewrite !(expr_eval_var_free _ _ ρ2 ρ1) by eauto;
+    eauto 10 using expr_typed_var_free.
+Qed.
+Global Instance assert_singleton_unlock_indep Γ e1 e2 malloc x τ :
+  perm_locked x = false → UnlockIndep (e1 ↦{malloc,x} e2 : τ).
+Proof.
+  intros ? Γ1 Δ1 ρ τs m ??? (a&v&?&?&?&?&?&?&?&->).
+  assert ((Γ1,Δ1) ⊢ v : τ ∧ (Γ1,Δ1) ⊢ a : TType τ ∧ addr_strict Γ1 a)
+    as (?&?&?) by eauto 15 using cmap_valid_memenv_valid, lval_typed_inv,
+    lval_typed_strict, rval_typed_inv, expr_eval_typed, cmap_empty_valid.
+  exists a v; split_ands; eauto using mem_unlock_all_singleton_unlocked.
+Qed.
+
+Lemma assert_singleton_union Γ e1 e2 malloc x y τ :
+  ⊥[x; y] → ¬sep_unmapped x → ¬sep_unmapped y →
+  (e1 ↦{malloc,x} e2 : τ ★ e1 ↦{malloc,y} e2 : τ)%A
+  ≡{Γ} (e1 ↦{malloc,x ∪ y} e2 : τ)%A.
+Proof.
+  intros; split.
+  * intros Γ1 Δ1 ρ τs ????? (?&?&->&?&(a1&v1&?&?&?&?&?&?&?&->)&
+      (a2&v2&?&?&?&?&?&?&?&->)); simplify_equality'.
+    assert ((Γ1,Δ1) ⊢ v1 : τ ∧ (Γ1,Δ1) ⊢ a1 : TType τ ∧ addr_strict Γ1 a1)
+      as (?&?&?) by eauto 15 using cmap_valid_memenv_valid, lval_typed_inv,
+      lval_typed_strict, rval_typed_inv, expr_eval_typed, cmap_empty_valid.
+    exists a1 v1; split_ands;
+      eauto 13 using mem_singleton_union, eq_sym, @sep_unmapped_union_l.
+  * intros Γ1 Δ1 ρ τs ????? (a&v&?&He1&?&?&He2&?&?&->).
+    assert (x ⊥ y) by solve_sep_disjoint.
+    assert ((Γ1,Δ1) ⊢ v : τ ∧ (Γ1,Δ1) ⊢ a : TType τ ∧ addr_strict Γ1 a)
+      as (?&?&?) by eauto 15 using cmap_valid_memenv_valid, lval_typed_inv,
+      lval_typed_strict, rval_typed_inv, expr_eval_typed, cmap_empty_valid.
+    exists (mem_singleton Γ1 a malloc x v) (mem_singleton Γ1 a malloc y v).
+    split_ands; rewrite ?sep_disjoint_list_double; solve
+      ltac:(eauto using mem_singleton_union, eq_sym, mem_singleton_disjoint).
+Qed.
+
+(* Lifting De Bruijn indexes *)
+Global Instance: Proper ((⊆{Γ}) ==> (⊆{Γ})) assert_lift.
+Proof. solve ltac:(eauto using Forall2_tail). Qed.
+Global Instance: Proper ((≡{Γ}) ==> (≡{Γ})) assert_lift.
+Proof. solve ltac:(eauto using Forall2_tail). Qed.
+
+Global Instance assert_lift_stack_indep: StackIndep P → StackIndep (P↑).
+Proof. solve ltac:(eauto using Forall2_tail). Qed.
+Global Instance assert_lift_unlock_indep: UnlockIndep P → UnlockIndep (P↑).
+Proof. solve ltac:(eauto using Forall2_tail). Qed.
+
+Lemma stack_indep_lift Γ P `{!StackIndep P} : (P↑)%A ≡{Γ} P.
+Proof. solve ltac:(eauto using Forall2_tail). Qed.
+Lemma assert_lift_impl Γ P Q : ((P → Q)↑)%A ≡{Γ} (P↑ → Q↑)%A.
+Proof. solve eauto. Qed.
+Lemma assert_lift_and Γ P Q : ((P ∧ Q)↑)%A ≡{Γ} (P↑ ∧ Q↑)%A.
+Proof. solve eauto. Qed.
+Lemma assert_lift_not Γ P : ((¬P)↑)%A ≡{Γ} (¬P↑)%A.
+Proof. solve eauto. Qed.
+Lemma assert_lift_forall Γ {A} (P : A → assert K) :
+  ((∀ x, P x)↑)%A ≡{Γ} (∀ x, P x↑)%A.
+Proof. solve eauto. Qed.
+Lemma assert_lift_exists Γ {A} (P : A → assert K) :
+  ((∃ x, P x)↑)%A ≡{Γ} (∃ x, P x↑)%A.
+Proof. solve eauto. Qed.
+Lemma assert_lift_sep Γ P Q : ((P ★ Q)↑)%A ≡{Γ} (P↑ ★ Q↑)%A.
+Proof. solve eauto. Qed.
+Lemma assert_lift_expr Γ e v τ : ((e ⇓ v : τ)↑)%A ≡{Γ} (e↑ ⇓ v : τ)%A.
+Proof.
+  split; repeat intro.
+  * do 2 red; by rewrite expr_eval_lift, expr_typed_lift.
+  * do 4 red; by rewrite <-expr_eval_lift, <-expr_typed_lift.
+Qed.
+Lemma assert_lift_expr_ Γ e τ : ((e ⇓ - : τ)↑)%A ≡{Γ} (e↑ ⇓ - : τ)%A.
+Proof. by rewrite assert_lift_exists; setoid_rewrite (assert_lift_expr Γ). Qed.
+Lemma assert_lift_singleton Γ e1 e2 malloc x τ :
+  ((e1 ↦{malloc,x} e2 : τ)↑)%A ≡{Γ} ((e1↑) ↦{malloc,x} (e2↑) : τ)%A.
+Proof.
+  split; repeat intro.
+  * do 2 red. by setoid_rewrite expr_eval_lift; setoid_rewrite expr_typed_lift.
+  * do 4 red; by setoid_rewrite <-expr_eval_lift;
+      setoid_rewrite <-expr_typed_lift.
+Qed.
+Lemma assert_lift_singleton_ Γ e1 malloc x τ :
+  ((e1 ↦{malloc,x} - : τ)↑)%A ≡{Γ} ((e1↑) ↦{malloc,x} - : τ)%A.
+Proof.
+  by rewrite assert_lift_exists; setoid_rewrite (assert_lift_singleton Γ);
+    setoid_rewrite lrval_to_expr_lift.
+Qed.
+
+(* Unlocking *)
+Global Instance: Proper ((⊆{Γ}) ==> (⊆{Γ})) assert_unlock.
+Proof. solve ltac:(eauto using mem_unlock_all_valid). Qed.
+Global Instance: Proper ((≡{Γ}) ==> (≡{Γ})) assert_unlock.
+Proof. solve ltac:(eauto using mem_unlock_all_valid). Qed.
+
+Lemma assert_unlock_unlock_indep Γ P `{!UnlockIndep P} : P ⊆{Γ} (P ○)%A.
+Proof. solve eauto. Qed.
+Lemma assert_unlock_impl Γ P Q : ((P → Q) ○)%A ≡{Γ} (P ○ → Q ○)%A.
+Proof.
+  split; [solve ltac:(eauto using mem_unlock_all_valid)|].
+  solve ltac:(eauto using cmap_valid_weaken_squeeze, mem_unlock_memenv_of).
+Qed.
+Lemma assert_unlock_and Γ P Q : ((P ∧ Q) ○)%A ≡{Γ} (P ○ ∧ Q ○)%A.
+Proof. solve eauto. Qed.
+Lemma assert_unlock_forall Γ {A} (P : A → assert K) :
+  ((∀ x, P x) ○)%A ≡{Γ} (∀ x, (P x) ○)%A.
+Proof. solve eauto. Qed.
+Lemma assert_unlock_exists Γ {A} (P : A → assert K) :
+  ((∃ x, P x) ○)%A ≡{Γ} (∃ x, (P x) ○)%A.
+Proof. solve eauto. Qed.
+Lemma assert_unlock_sep Γ P Q : (P ○ ★ Q ○)%A ⊆{Γ} ((P ★ Q) ○)%A.
+Proof.
+  intros Γ1 Δ1 ρ τs m ???? (m1&m2&->&?&?&?).
+  exists (mem_unlock_all m1) (mem_unlock_all m2); split_ands; auto.
+  * by rewrite mem_unlock_all_union by solve_sep_disjoint.
+  * by rewrite <-!mem_unlock_all_disjoint_le.
+Qed.
+Lemma assert_unlock_sep_alt Γ P P' Q Q' :
+  P ⊆{Γ} (P' ○)%A → Q ⊆{Γ} (Q' ○)%A → (P ★ Q)%A ⊆{Γ} ((P' ★ Q') ○)%A.
+Proof. intros HP HQ. by rewrite HP, HQ, assert_unlock_sep. Qed.
+
+Lemma assert_unlock_singleton Γ e1 e2 malloc x τ :
+  perm_locked x = true →
+  (e1 ↦{malloc,x} e2 : τ)%A ⊆{Γ} ((e1 ↦{malloc,perm_unlock x} e2 : τ) ○)%A.
+Proof.
+  intros ? Γ1 Δ1 ρ τs m ???? (a&v&?&?&?&?&?&?&?&->).
+  exists a v; split_ands; eauto using perm_unlock_valid, perm_unlock_mapped.
+  assert ((Γ1,Δ1) ⊢ v : τ ∧ (Γ1,Δ1) ⊢ a : TType τ ∧ addr_strict Γ1 a)
+    as (?&?&?) by eauto 15 using cmap_valid_memenv_valid, lval_typed_inv,
+    lval_typed_strict, rval_typed_inv, expr_eval_typed, cmap_empty_valid.
+  by erewrite mem_unlock_all_singleton by eauto.
+Qed.
+Lemma assert_unlock_singleton_ Γ e1 malloc x τ :
+  perm_locked x = true →
+  (e1 ↦{malloc,x} - : τ)%A ⊆{Γ} ((e1 ↦{malloc,perm_unlock x} - : τ) ○)%A.
+Proof.
+  intros Hx. rewrite assert_unlock_exists.
+  by setoid_rewrite (λ e2, assert_unlock_singleton Γ e1 e2 malloc x τ Hx).
+Qed.
+Lemma assert_lock_singleton Γ e1 e2 malloc x τlr :
+  sep_valid x → Some Writable ⊆ perm_kind x →
+  (e1 ↦{malloc,perm_lock x} e2 : τlr)%A ⊆{Γ} ((e1 ↦{malloc,x} e2 : τlr) ○)%A.
+Proof.
+  intros. by rewrite assert_unlock_singleton,
+    perm_unlock_lock by auto using perm_locked_lock.
+Qed.
+Lemma assert_lock_singleton_ Γ e1 malloc x τlr :
+  sep_valid x → Some Writable ⊆ perm_kind x →
+  (e1 ↦{malloc,perm_lock x} - : τlr)%A ⊆{Γ} ((e1 ↦{malloc,x} - : τlr) ○)%A.
+Proof.
+  intros. by rewrite assert_unlock_singleton_,
+    perm_unlock_lock by auto using perm_locked_lock.
+Qed.
+End assertions.
